\documentclass{article}
\usepackage{amsmath}

\begin{document}

\section{Introduction}

\begin{equation}
\label{eq:recourse}
\ell(f_i(x), 1) + \lambda \, c(x_z, x)
\end{equation}

\begin{equation}
\ell(f_i(x), 1) = (1 - f_i(x))^2
\end{equation}

\begin{equation}
f_i(x) = (1-\frac{1}{1+e^{w^T x}})^2
\end{equation}

\begin{equation}
(1-\frac{1}{1+e^{w^T x}})^2 + \lambda c(x_z, x)
\end{equation}

\begin{equation}
c(x_z, x) = \|x_z - x\|^2 
\end{equation}

\begin{equation}
(1-\frac{1}{1+e^{w^T x}})^2 + \lambda =\|x_z - x\|^2 
\end{equation}

\begin{align}
f(x) = \frac{d}{dx}(1-\frac{1}{1+e^{w^T x}})^2 + \lambda \|x_z - x\|^2 \\ 
\end{align}

\begin{align}
f'(x)= 2 \cdot \frac{-we^{w^Tx}}{ (1 + e^{w^T x})^2 } \cdot (1-\frac{1}{1+e^{w^T x}})^2 + -2\lambda (x_z - x)
\end{align}

\begin{align}
f''(x) = \frac{2 \left({\lambda}\mathrm{e}^{4w^{T} x} + \left(4{\lambda} - w^{2T}\right) \mathrm{e}^{3w^{T} x} + \left(6{\lambda} + 2w^{2T}\right) \mathrm{e}^{2w^{T} x} + 4{\lambda}\mathrm{e}^{w^{T} x} + {\lambda}\right)}{\left(\mathrm{e}^{w^{T} x} + 1\right)^{4}}
\end{align}

Two colleges:

\begin{equation}
f(x)=1-\Pi_{i=1}^n(1-f_i(x)),
\end{equation}

\end{document}

